

\magnification=1200
\baselineskip=14pt

\def\A {{\bf A}} 
\def\B {{\cal B}}
\def\C {{\bf C}}
\def\CC {{\cal C}}
\def\Cl {{\tt \hbox{Cliff}}}
\def\E {{\bf E}}
\def\EE {{\cal E}}
\def\F {{\cal F}}
\def\FF {{\cal F}}
\def\G {\Gamma}
\def\GG {{\cal G}}
\def\H {{\bf H}}
\def\K {{\bf K}}
\def\L {{\cal L}}
\def\M {{\cal M}}
\def\N {{\bf N}}
\def\R {{\bf R}}
\def\Sb {{\bf S}}
\def\SS {{\cal S}}
\def\Tr {{\rm Tr\,}}
\def\V {{\cal V}}
\def\X {{\bf X}}
\def\XX {{\cal X}}
\def\Y {{\bf Y}}
\def\Z {{\bf Z}}

\def\a {\alpha}
\def\ac {{\bf a}}
\def\b {{\bf b}}
\def\bs {{\bf s}}
\def\c {{\bf c}}
\def\d {\delta}
\def\dist {{\tt \hbox{distance}}}
\def\e {{\bf e}}
\def\f {{\bf f}}
\def\finish {\blacksquare}
\def\g {{\bf g}}
\def\grad {{\rm grad\,}}
\def\h {\hbar}
\def\k {{\bf k}}
\def\l {{\bf l}}
\def\m {{\bf m}}
\def\n {{\bf n}}
\def\p {\partial}
\def\pb {{\bf p}}
\def\pt {{\bf pt}}
\def\q {{\bf q}}
\def\r {{\bf r}}
\def\s {\sigma}
\def\t {{\bf t}}
\def\tS {{\tilde \Sigma}}
\def\td {\tilde}
\def\v {{\bf v}}
\def\vare {\varepsilon}
\def\x {{\bf x}}
\def\y {{\bf y}}
\def\w {\omega}


\centerline{\bf One way to define thick morphisms}

  Let $M=\R^m$, $N=\R^n$ be two linear spaces.
 Consider a function $S(x,q)$ where $x\in M$ and $q\in
T^*N$ such that
      $$
S(x,q)=S_0(x)+\varphi^i(x)q_i+S_+(x,q)
      $$
where $S_+$ possesses terms of order by $q$
higher or equal than $2$:
        $$
S_+(x,q)={1\over 2}\Pi^{ij}(x)q_iq_j+
{1\over 6}\Pi^{ijk}(x)q_iq_jq_k+\dots
        $$
Define the action of (quantum) thick morphism   
  We have
      $$
      \Phi_S^*(w(y))=\Psi(x)=
    \int
e^{
{i\over \hbar}
    \left(S(x,q)-y^iq_i\right)}
      w(y)
      dydq=
     \int 
      e^{
{i\over \hbar}
    S(x,q)}
      \bar w(q)
        dq\,,
          $$
where $\bar w(q)$ is Fourrier image of function $w(y)$:
        $$
\bar w(q)=\int w(y)e^{-{i\over \hbar}qy}dy\,\quad {\rm
and} \quad
 w(y)=\int \bar w(q)e^{{i\over \hbar}qy}dq,,
\hbox {(up to multiplier)}\,.
        $$
Now use the standard identity that up to multiplier
            $$
         f(q)
      \bar w(q)=
       \int   
       \left[
    f\left({\hbar\over i}{\p\over \p y}\right)w(y)
    \right]
      e^{-{i\over \hbar}qy}dy\,.
           $$
Indeed
            $$
         f(q)
      \bar w(q)=
      \int
       f(k)
      \bar w(k)\delta (k-q)dk= 
      \int
         f(k)
      \bar w(k) e^{{i\over \hbar}(k-q)y}dkdy= 
       $$
        $$
      \int
        \left[
     f\left(
  {\hbar\over i}{\p\over \p y}
       \right)   
       e^{{i\over \hbar}ky}\bar w(k)
         \right]   
    e^{-{i\over \hbar}qy}dkdy=   
      \int
        \left[
     f\left(
  {\hbar\over i}{\p\over \p y}
       \right)   
w(y)         
\right]   
    e^{-{i\over \hbar}qy}dy\,.
   $$ 
Hence
            $$
  \Phi_S^*(w(y))=\Psi(x)=
    \int
e^{
{i\over \hbar}
    \left(S(x,q)-y^iq_i\right)}
      w(y)
      dydq=
     \int 
      e^{
{i\over \hbar}
    S(x,q)}
      \bar w(q)
        dq=
         $$
         $$
        \int
     \left( 
       e^{
{i\over \hbar}
    S(\left(x,{\hbar\over i}{\p\over \p y}\right)}
      w(y)
      \right)
        e^{-iqy}
        dydq=
        $$
        $$
      \left( 
       e^{
{i\over \hbar}
    S(\left(x,{\hbar\over i}{\p\over \p y}\right)}
      w(y)
      \right)
       \delta(y)
       dy
        =
     \left( 
       e^{
{i\over \hbar}
    S(\left(x,{\hbar\over i}{\p\over \p y}\right)}
      w(y)
      \right)
       \big\vert_{y=0}
       $$
       $$
      \left( 
       e^{
{i\over \hbar}
     \left(
         S_0(x)
                +
          \varphi(x){\hbar\over i}{\p\over \p y}
            +
    S_+\left(x,{\hbar\over i}{\p\over \p y}\right)
     \right)
      }
      w(y)
      \right)
       \big\vert_{y=0}
        =
          e^{{i\over \hbar}S_0(x)}
      \left(
        e^{\varphi(x){\p\over \p y}} 
       e^{
{i\over \hbar}
    S_+\left(x,{\hbar\over i}{\p\over \p y}\right)
      }
      w(y)
      \right)
       \big\vert_{y=0}
        =
        $$
$$ 
\left( 
       e^{
{i\over \hbar}
   S_+\left(x,{\hbar\over i}{\p\over \p y}\right)
      }
      w(y)
      \right)
       \big\vert_{y=\varphi(x)}\,.
 \eqno (1)
$$
We suppose here that $S_0(x)\equiv 0$.


One can consider the one-parametric family $L^*_\hbar$

          $$
  L^*_\hbar (g(y))=f(x)\,, \hbox {such that}\,\,
      \Psi(x)=e^{{i\over \hbar}f(x)}=
    \Phi_S^*\left(
e^{{i\over \hbar}g(y)}
        \right)\,,
     \eqno (2)
          $$
and its limit
          $$
       L^*_{S \rm classic.}(g(y))=\lim_{\hbar\to 0}
  L^*_\hbar (g(y))\,.
  \eqno (2a)
          $$
One can see that this is a la `Legendre':
            $$
       L^*_{\rm classic.}(g(y))=
        S(x,q)+g(y)-y^iq_i\,,
           $$
where
             $$
           y^i={\p S(x,q)\over \p q_i}=
    \varphi^i(x)+\Pi^{ij}(x)q_j
        +\Pi^{ijk}(x)q_j+\dots\,\,\hbox {such that}\,\,
       q_i={\p g(y)\over \p y^i}\,,.
            $$ 

Here we have to be carefull taking limits.

    Calculate (2):
 $$
  L^*_\hbar (g(y))=
      f(x)=
       {\hbar\over i} 
     \log
      \left(\Psi(x)\right)= 
      {\hbar\over i} 
     \log
      \left( \Phi_S^*\left(
e^{{i\over \hbar}g(y)}
        \right)
         \right)=
             $$
              $$
      {\hbar\over i} 
     \log
      \left( 
 e^{{i\over \hbar}S_+\left(x, {\hbar\over i}{\p\over \p y}\right)}
\left(
e^{{i\over \hbar}g(y)}
        \right)
         \right)\big\vert_{y=\varphi(x)}=
                $$
              $$
      {\hbar\over i} 
     \log
         \left[
 e^{{i\over \hbar}g(y)}
         \left\{
 e^{-{i\over \hbar}g(y)}
      \left( 
 e^{{i\over \hbar}S_+\left(x, {\hbar\over i}{\p\over \p y}\right)}
\left(
e^{{i\over \hbar}g(y)}
        \right)
         \right)
         \right\}
\right]
 \big\vert_{y=\varphi(x)}=
                $$
     $$
      {\hbar\over i} 
         \left[
   { {i\over \hbar}g(y)}
          +\log
         \left\{
 e^{-{i\over \hbar}g(y)}
      \left( 
 e^{{i\over \hbar}S_+\left(x, {\hbar\over i}{\p\over \p y}\right)}
\left(
e^{{i\over \hbar}g(y)}
        \right)
         \right)
         \right\}
\right]
 \big\vert_{y=\varphi(x)}=
                $$
     $$
         \left[
               g(y)
          +{\hbar\over i}
           \log
         \left\{
 e^{-{i\over \hbar}g(y)}
      \left( 
 e^{{i\over \hbar}S_+\left(x, {\hbar\over i}{\p\over \p y}\right)}
\left(
e^{{i\over \hbar}g(y)}
        \right)
         \right)
         \right\}
\right]
 \big\vert_{y=\varphi(x)}=
                $$
                 $$
         \left[
               g(y)
          +{\hbar\over i}
           \log
         \left\{
 e^{-{i\over \hbar}g(y)}
      \left( 
 e^{{i\over \hbar}S_+\left(x, {\hbar\over i}{\p\over \p y}\right)}
\left(
e^{{i\over \hbar}g(y)}
        \right)
         \right)
         \right\}
\right]
 \big\vert_{y=\varphi(x)}=
                $$
                   $$
         \left[
               g(y)
          +{\hbar\over i}
           \log
         \left\{
   e^{{i\over \hbar}S_+\left(x, {\p g\over \p y}\right)}
   +\dots
         \right\}
\right]
 \big\vert_{y=\varphi(x)}\,,
                \eqno (3)
                $$
where we denote by dots the terms of 
order equal or higher than zero by $\hbar$.

Ochenj khochetsia zakljuchitj iz etoj formuly shto
 for classical thick morphisms
         $$
  \Phi_S(g(y))= f(x)=\lim_{\hbar\to 0} f_\hbar(x)=
       \lim_{\hbar\to 0}  \left[
               g(y)
          +{\hbar\over i}
           \log
         \left\{
   e^{{i\over \hbar}S_+\left(x, {\p g\over \p y}\right)}
   +O(1)
         \right\}
\right]
 \big\vert_{y=\varphi(x)} = 
\eqno (3a) 
      $$
                    $$
   \left(g(y)+S_+\left(x, {\p g\over \p y}\right)\right)
\big\vert_{y=\varphi(x)}\,.
          $$

No eto zhe ne tak!

We have to  look on (3) more carefully
     

\bye
