

\magnification=1200
\baselineskip=14pt
\def\vare {\varepsilon}
\def\t {\tilde}
\def\a {\alpha}
\def\K {{\bf K}}
\def\N {{\bf N}}
\def\C {{\bf C}}
\def\L {{\cal L}}
\def\E {{\bf E}}
\def\s {{\sigma}}
\def\S {{\cal S}}
\def\SS {{\Sigma}}
\def\p{\partial}
\def\vare{{\varepsilon}}
\def\Q {{\bf Q}}
\def\D {{\cal D}}
\def\A {{\cal A}}
\def\B {{\cal B}}
\def\G {{\Gamma}}
\def\Z {{\bf Z}}
\def\R  {{\bf R}}
\def\l {\lambda}
\def\ll {{\bf l}}
\def\degree {{\bf {\rm degree}\,\,}}
\def \finish {${\,\,\vrule height1mm depth2mm width 8pt}$}
\def \m {\medskip}
\def\p {\partial}
\def\r {{\bf r}}
\def\pt {{\bf p}}
\def\v {{\bf v}}
\def\n {{\bf n}}
\def\t {{\bf t}}
\def\b {{\bf b}}
\def\c {{\bf c }}
\def\e{{\bf e}}
\def\f{{\bf f}}
\def\ac {{\bf a}}
\def \X   {{\bf X}}
\def \Y   {{\bf Y}}
\def \x   {{\bf x}}
\def \y   {{\bf y}}
\def\w {{\omega}}
\def \Tr  {{\rm Tr\,}}
\def\dim {{\rm dim\,\,}}
% I wrote this file on 16 January
\def\t {{\tilde}} 
\def\dist {{\hbox{\tt "distance"}}}
\def  \dim {{\rm dim\,}}
\def  \Im  {{\rm Im\,}}
\def  \ker {{\rm ker\,}}


\def \Cl {\hbox{\tt Cliff}}
\def\F {\cal F}

\centerline {\bf Composition of  morphisms}


Let $S_1=S_1(x,p)$ be action of thick morphism $M\to N$
and  $S_2(y,t)$  be the action of thick morphism from
$N\to R$, and let $S_{13}=S_{13}(x,t)$ be the action of
composition of these morphisms. Let $h$ be a function on
$R$, $g(y)=\Phi^*_{23}h$ and $f(x)=\Phi^*_{12}g$ and
          $$
     e^{{i\over \hbar}f(x)}=
\int e^{{i\over \hbar}(S_{13}(x,t)-zt+h(z))}DtDz=
\int e^{{i\over \hbar}(S_{12}(x,q)-yq+g(y))}DqDy\,,
          $$
and
          $$
     e^{{i\over \hbar}g(y)}=
\int e^{{i\over \hbar}(S_{23}(y,t)-zt+h(z))}DtDz=
          $$
hence

          $$
     e^{{i\over \hbar}f(x)}=
\int e^{{i\over \hbar}(S_{13}(x,t)-zt+h(z))}DtDz=
\int e^{{i\over \hbar}(S_{12}(x,q)-yq+g(y))}DqDy=
        $$
        $$
\int e^{{i\over \hbar}(S_{12}(x,q)-yq+
  S_{23}(y,t)-zt+h(z))}DtDzDqDy\,,
          $$
Thus we see that
    $$
 e^{{i\over \hbar}S_{13}(x,t}=
 \int e^{{i\over
\hbar}(S_{12}(x,q)+S_{23}(y,t)-yq}DyDq\,,
    \eqno (1)
    $$
i.e. for classical case 
       $$
S_{13}(x,t)=S_{12}(x,q)+S_{23}(y,t)-yq\,. 
      $$
and it does not depend on  $y$, $q$, i.e.
       $$
{\p S_{12}(x,q)\over \p q}-y=
{\p S_{23}(y,t)\over \p y}-q=0\,.
       $$

For quantum morphisms we have to consider the integral
 (1).

Consider the special cases

 1) $S_{23}(y,t)=g(y)t$, i.e. the second morphism is
usual one.

  In this case
         $$
  S_{13}(x,t)=S_{12}(x,y)+g(y)q-yq
         $$
and one can see that
       $$
     \Phi_{13}^*(z)=\Phi_{12}^*g
       $$

2)  First and second morphisms are quadratic.  Then

    $$
 e^{{i\over \hbar}S_{13}(x,t}=
 \int e^{{i\over
\hbar}(S_{12}(x,q)+S_{23}(y,t)-yq}DyDq=
    $$
         $$
             \int e^{
           {i\over \hbar}
             \left(
   {1\over 2}x^a a_{ab}x^b+x^a\A_a^iq_i+
     {1\over 2}A^{ij}q_iq_j +
    {1\over 2}y^ib_{ij}y^j+
  y^i\B_i^\a t_\a+
 {1\over 2}B^{\a\beta}t_\a t_\beta 
                  -y^iq_i
            \right)
                   }
      DyDq\,,
\eqno (3)
    $$
Classicaly
    $$
   \cases
       {
 y^i=\A^i_a x^a+A^{ij}q_j\cr
 q_i= \B_i^\a t_\a+b_{ij}y^j\cr
      }
    \Rightarrow
     \cases
       {
y=(1-Ab)^{-1}(\A x+A\B t)\cr
q=(1-bA)^{-1}(\B t+ b\A x)\cr        
      }
    $$

      $$
S_{13}(x,t)=S_{12}(x,q)+S_{23}(y,t)-yq
\quad  (y=\dots, q=\dots)\,.
      $$


For quantum case we have to calculate (3).
Rewrite it (we change little bit notations)
            $$
 e^{{i\over \hbar}S_{13}(x,t}=
 \int e^{{i\over
\hbar}
     (S_{12}(x,q)+S_{23}(y,t)-yq}DyDq=
    $$
         $$
             \int e^{
           {i\over \hbar}
            \left(
  {1\over 2} x^a a_{ab}x^b+x^a\A_a^iq_i+
    {1\over 2}A^{ij}q_iq_j +
    {1\over 2}
 y^ib_{ij}y^j+
  y^i\B_i^\a t_\a+
  {1\over 2}B^{\a\beta}t_\a t_\beta 
                  -y^iq_i
             \right)
                   }
      DyDq=
    $$
          $$
             \int 
            \exp
          {
           {i\over \hbar}
            \left(
  {1\over 2} x^a a_{ab}x^b+x^a\A_a^i \tilde {q_i}+
    {1\over 2}A^{ij}\tilde {q_i}
       \tilde {q_j} +
    {1\over 2}
 \tilde {y^i}b_{ij}\tilde {y^j}+
  \tilde {y^i}\B_i^\a t_\a+
  {1\over 2}B^{\a\beta}t_\a t_\beta 
                  -\tilde {y^i}\tilde {q_i}
             \right)
                   }
      D\tilde yD\tilde q=
    $$     

Now we change $\tilde q=q+\beta$, $\tilde y=y+\a$
     $$
 \int DqDp \exp{i\over \hbar}
     \left(  \right.
           $$
           $$
       \left.
  {1\over 2} x ax+x\A  (q+\beta)+
    {1\over 2}A (q+\beta)(q+\beta)
               +
    {1\over 2}
 (y+\a)b (y+\a)+
  (y+\a)\B t+
  {1\over 2}Bt t 
                  -(y+\a) (q+\beta)
             \right)
    $$
      $$
 =\int DqDp \exp{i\over \hbar}
     \left(  \right.
           $$
Now we choose  $\a$ and $\beta$ such that
       $$
    \cases
 {
   \A x+A\beta=\a\cr
          v\a+\B t=\beta\cr  
 }
 \Rightarrow
 \cases
 {
   \a=(1-Ab)^{-1}(\A x+ A \B t)\cr
  \beta=(1-bA)^{-1}(\B t+ b\A x)\cr  
 }
       $$
In this way we will eliminate all the terms which are
linear by $q$ and $y$. We will come to
      $$
 =\int DqDp \exp{i\over \hbar}
     \left(  \right.
           $$
       $$
       \left.
  {1\over 2} x^a a_{ab} x^b+
    {1\over 2}A^{ij} q_iq_j+
    {1\over 2}
        b_{ij}y^iy^j-y^iq_i+
    {1\over 2}B^{\a\beta}t_{\a}t_\beta
       +\right.
         $$
         $$
      \left.
         +
  \A^i_a x^a\beta_i+
{1\over 2}A^{ij}
\beta_i\beta_j+
{1\over 2}b_{ij}
\a^i\a^j+
  \B^\a_i \a^i t_\a-\a^i\beta_i
             \right)=
    $$
    $$
     {C\over 
       \sqrt
        {
        \det
       \left(
      {1\over 2} 
        \pmatrix
         {
      b_{ij} & -1\cr
      -1 &    A^{ij}\cr
         }
           \right)
       }
      }
 \exp {i\over \hbar}
    \left(
  {1\over 2} x^a a_{ab} x^b+
    {1\over 2}B^{\a\beta}t_{\a}t_\beta
       +\right)
     $$
      $$
 \exp {i\over \hbar}
 \left(
  \A^i_a x^a\beta_i+
{1\over 2}A^{ij}
\beta_i\beta_j+
{1\over 2}b_{ij}
\a^i\a^j+
  \B^\a_i \a^i t_\a-\a^i\beta_i
\right)\,,
      $$
 where $\a^i$ and $\beta_j$ are defined above.   

   \bye
